compiler/backend/passes/pure_comp_confScript.sml
@@ -7,31 +7,47 @@ open HolKernel Parse boolLib bossLib mlstringTheory;
 val _ = new_theory "pure_comp_conf";
 
 Datatype:
+  inline_opts = <|
+    depth           : num ;
+    heuristic       : num ;
+  |>
+End
+
+Datatype:
   compiler_opts = <|
-      do_pure_sort  : bool ;  (* pure-to-pure binding group analysis *)
-      do_pure_clean : bool ;  (* pure-to-pure cleaning / deadcode elimination *)
-      do_demands    : bool ;  (* demand analysis *)
-      do_mk_delay   : bool ;  (* thunk-to-thunk smart mk_delay constructor *)
-      do_let_force  : bool ;  (* thunk-to-thunk simplify let force *)
-      do_split_dlam : bool ;  (* thunk-to-thunk split delayed lambdas *)
-      do_app_unit   : bool ;  (* state-to-state *)
-      do_final_gc   : bool ;  (* invoke GC at end of CakeML program *)
+      do_pure_sort  : bool ;        (* pure-to-pure binding group analysis *)
+      do_pure_clean : bool ;        (* pure-to-pure cleaning / deadcode elimination *)
+      do_demands    : bool ;        (* demand analysis *)
+      inlining      : inline_opts ; (* inlining *)
+      do_mk_delay   : bool ;        (* thunk-to-thunk smart mk_delay constructor *)
+      do_let_force  : bool ;        (* thunk-to-thunk simplify let force *)
+      do_split_dlam : bool ;        (* thunk-to-thunk split delayed lambdas *)
+      do_app_unit   : bool ;        (* state-to-state *)
+      do_final_gc   : bool ;        (* invoke GC at end of CakeML program *)
     |>
 End
 
 Overload pure_sort_flag[local]  = “strlit "-sort"”
 Overload pure_clean_flag[local] = “strlit "-clean"”
 Overload demands_flag[local]    = “strlit "-demands"”
+Overload inline_off_flag[local] = “strlit "-inline"”
+Overload inline_max_flag[local] = “strlit "-inline_max"”
 Overload mk_delay_flag[local]   = “strlit "-mk_delay"”
 Overload let_force_flag[local]  = “strlit "-let_force"”
 Overload dlam_flag[local]       = “strlit "-dlam"”
 Overload unit_flag[local]       = “strlit "-unit"”
 Overload final_gc_flag[local]   = “strlit "-final_gc"”
 
+Overload inline_off_opts[local] = “<| depth := 0 ; heuristic := 0 |>”
+Overload inline_default_opts[local] = “<| depth := 50 ; heuristic := 100 |>”
+Overload inline_max_opts[local] = “<| depth := 5000 ; heuristic := 10000 |>”
+
 Definition all_flags_def:
   all_flags = [pure_sort_flag;
                pure_clean_flag;
                demands_flag;
+               inline_off_flag;
+               inline_max_flag;
                mk_delay_flag;
                let_force_flag;
                dlam_flag;
@@ -46,6 +62,11 @@ Definition read_cline_args_def:
     | [] => INL <| do_pure_sort  := ¬ MEM pure_sort_flag cl  ;
                    do_pure_clean := ¬ MEM pure_clean_flag cl ;
                    do_demands    := ¬ MEM demands_flag cl    ;
+                   inlining      := if MEM inline_off_flag cl then
+                                      inline_off_opts
+                                    else if MEM inline_max_flag cl then
+                                      inline_max_opts
+                                    else inline_default_opts ;
                    do_mk_delay   := ¬ MEM mk_delay_flag cl   ;
                    do_let_force  := ¬ MEM let_force_flag cl  ;
                    do_split_dlam := ¬ MEM dlam_flag cl       ;
